<?xml version="1.0"?>
<rdf:RDF xmlns="https://w3id.org/mdo/core/"
     xml:base="https://w3id.org/mdo/core/"
     xmlns:owl="http://www.w3.org/2002/07/owl#"
     xmlns:rdf="http://www.w3.org/1999/02/22-rdf-syntax-ns#"
     xmlns:xml="http://www.w3.org/XML/1998/namespace"
     xmlns:xsd="http://www.w3.org/2001/XMLSchema#"
     xmlns:emmo="http://emmo.info/domains/emmo-material.owl#"
     xmlns:rdfs="http://www.w3.org/2000/01/rdf-schema#"
     xmlns:vann="http://purl.org/vocab/vann/"
     xmlns:dcterms="http://purl.org/dc/terms/">
    <owl:Ontology rdf:about="https://w3id.org/mdo/core/">
        <owl:versionIRI rdf:resource="https://w3id.org/mdo/core/1.0"/>
        <dcterms:contributor rdf:datatype="http://www.w3.org/2001/XMLSchema#string">Patrick Lambrix</dcterms:contributor>
        <dcterms:contributor rdf:datatype="http://www.w3.org/2001/XMLSchema#string">Rickard Armiento</dcterms:contributor>
        <dcterms:created>2019-11-07</dcterms:created>
        <dcterms:creator rdf:datatype="http://www.w3.org/2001/XMLSchema#string">Huanyu Li</dcterms:creator>
        <dcterms:license>https://github.com/huanyu-li/Materials-Design-Ontology/blob/master/LICENSE</dcterms:license>
        <dcterms:title xml:lang="en">Materials Design Ontology - Core Module</dcterms:title>
        <vann:preferredNamespacePrefix>core</vann:preferredNamespacePrefix>
        <vann:preferredNamespaceUri>https://w3id.org/mdo/core/1.0</vann:preferredNamespaceUri>
        <rdfs:comment xml:lang="en">This is the core module in Materials Design Ontology.</rdfs:comment>
        <rdfs:seeAlso>https://github.com/huanyu-li/Materials-Design-Ontology</rdfs:seeAlso>
        <owl:versionInfo rdf:datatype="http://www.w3.org/2001/XMLSchema#string">1.0</owl:versionInfo>
    </owl:Ontology>
    


    <!-- 
    ///////////////////////////////////////////////////////////////////////////////////////
    //
    // Annotation properties
    //
    ///////////////////////////////////////////////////////////////////////////////////////
     -->

    


    <!-- http://purl.org/dc/terms/contributor -->

    <owl:AnnotationProperty rdf:about="http://purl.org/dc/terms/contributor"/>
    


    <!-- http://purl.org/dc/terms/created -->

    <owl:AnnotationProperty rdf:about="http://purl.org/dc/terms/created"/>
    


    <!-- http://purl.org/dc/terms/creator -->

    <owl:AnnotationProperty rdf:about="http://purl.org/dc/terms/creator"/>
    


    <!-- http://purl.org/dc/terms/license -->

    <owl:AnnotationProperty rdf:about="http://purl.org/dc/terms/license"/>
    


    <!-- http://purl.org/dc/terms/title -->

    <owl:AnnotationProperty rdf:about="http://purl.org/dc/terms/title"/>
    


    <!-- http://purl.org/vocab/vann/preferredNamespacePrefix -->

    <owl:AnnotationProperty rdf:about="http://purl.org/vocab/vann/preferredNamespacePrefix"/>
    


    <!-- http://purl.org/vocab/vann/preferredNamespaceUri -->

    <owl:AnnotationProperty rdf:about="http://purl.org/vocab/vann/preferredNamespaceUri"/>
    


    <!-- 
    ///////////////////////////////////////////////////////////////////////////////////////
    //
    // Datatypes
    //
    ///////////////////////////////////////////////////////////////////////////////////////
     -->

    


    <!-- http://www.w3.org/2001/XMLSchema#date -->

    <rdfs:Datatype rdf:about="http://www.w3.org/2001/XMLSchema#date"/>
    


    <!-- 
    ///////////////////////////////////////////////////////////////////////////////////////
    //
    // Object Properties
    //
    ///////////////////////////////////////////////////////////////////////////////////////
     -->

    


    <!-- https://w3id.org/mdo/core/hasInputProperty -->

    <owl:ObjectProperty rdf:about="https://w3id.org/mdo/core/hasInputProperty">
        <rdfs:domain rdf:resource="https://w3id.org/mdo/core/Calculation"/>
        <rdfs:range rdf:resource="https://w3id.org/mdo/core/Property"/>
        <rdfs:comment xml:lang="en">hasInputProperty represents the relationship between a calculation and the properties it takes as input.</rdfs:comment>
    </owl:ObjectProperty>
    


    <!-- https://w3id.org/mdo/core/hasInputStructure -->

    <owl:ObjectProperty rdf:about="https://w3id.org/mdo/core/hasInputStructure">
        <rdfs:domain rdf:resource="https://w3id.org/mdo/core/Calculation"/>
        <rdfs:range rdf:resource="https://w3id.org/mdo/core/Structure"/>
        <rdfs:comment xml:lang="en">hasInputStructure represents the relationship between a calculation and the structures it takes as input.</rdfs:comment>
    </owl:ObjectProperty>
    


    <!-- https://w3id.org/mdo/core/hasOutputCalculatedProperty -->

    <owl:ObjectProperty rdf:about="https://w3id.org/mdo/core/hasOutputCalculatedProperty">
        <rdfs:domain rdf:resource="https://w3id.org/mdo/core/Calculation"/>
        <rdfs:range rdf:resource="https://w3id.org/mdo/core/CalculatedProperty"/>
        <rdfs:comment xml:lang="en">hasOutputCalculatedProperty represents the relationship between a calculation and the calculated properties it outputs.</rdfs:comment>
    </owl:ObjectProperty>
    


    <!-- https://w3id.org/mdo/core/hasOutputStructure -->

    <owl:ObjectProperty rdf:about="https://w3id.org/mdo/core/hasOutputStructure">
        <rdfs:domain rdf:resource="https://w3id.org/mdo/core/Calculation"/>
        <rdfs:range rdf:resource="https://w3id.org/mdo/core/Structure"/>
        <rdfs:comment xml:lang="en">hasOutputStructure represents the relationship between a calculation and the structures it outputs.</rdfs:comment>
    </owl:ObjectProperty>
    


    <!-- https://w3id.org/mdo/core/relatesToMaterial -->

    <owl:ObjectProperty rdf:about="https://w3id.org/mdo/core/relatesToMaterial">
        <rdfs:domain rdf:resource="https://w3id.org/mdo/core/Structure"/>
        <rdfs:range rdf:resource="http://emmo.info/domains/emmo-material.owl#EMMO_4207e895_8b83_4318_996a_72cfb32acd94"/>
        <rdfs:comment xml:lang="en">relatesToMaterial represents the relationship between a structure and the materials it comes from.</rdfs:comment>
    </owl:ObjectProperty>
    


    <!-- https://w3id.org/mdo/core/relatesToStructure -->

    <owl:ObjectProperty rdf:about="https://w3id.org/mdo/core/relatesToStructure">
        <rdfs:domain rdf:resource="https://w3id.org/mdo/core/Property"/>
        <rdfs:range rdf:resource="https://w3id.org/mdo/core/Structure"/>
        <rdfs:comment xml:lang="en">relatesToStructure represents the relationship between a property and the structures it comes from.</rdfs:comment>
    </owl:ObjectProperty>
    


    <!-- 
    ///////////////////////////////////////////////////////////////////////////////////////
    //
    // Data properties
    //
    ///////////////////////////////////////////////////////////////////////////////////////
     -->

    


    <!-- https://w3id.org/mdo/core/hasID -->

    <owl:DatatypeProperty rdf:about="https://w3id.org/mdo/core/hasID">
        <rdfs:domain rdf:resource="https://w3id.org/mdo/core/Calculation"/>
        <rdfs:range rdf:resource="http://www.w3.org/2001/XMLSchema#string"/>
        <rdfs:comment xml:lang="en">hasID represents that a calculation has the unique ID in a string.</rdfs:comment>
    </owl:DatatypeProperty>
    


    <!-- https://w3id.org/mdo/core/hasPropertyName -->

    <owl:DatatypeProperty rdf:about="https://w3id.org/mdo/core/hasPropertyName">
        <rdfs:domain rdf:resource="https://w3id.org/mdo/core/Property"/>
        <rdfs:range rdf:resource="http://www.w3.org/2001/XMLSchema#string"/>
        <rdfs:comment xml:lang="en">hasPropertyName represents that a property has the name in a string.</rdfs:comment>
    </owl:DatatypeProperty>
    


    <!-- https://w3id.org/mdo/core/hasPropertyValue -->

    <owl:DatatypeProperty rdf:about="https://w3id.org/mdo/core/hasPropertyValue">
        <rdfs:domain rdf:resource="https://w3id.org/mdo/core/Property"/>
        <rdfs:range rdf:resource="http://www.w3.org/2001/XMLSchema#double"/>
        <rdfs:comment xml:lang="en">hasPropertyValue represent that a property has the value in a double.</rdfs:comment>
    </owl:DatatypeProperty>
    


    <!-- https://w3id.org/mdo/core/hasUnit -->

    <owl:DatatypeProperty rdf:about="https://w3id.org/mdo/core/hasUnit">
        <rdfs:domain rdf:resource="https://w3id.org/mdo/core/Property"/>
        <rdfs:range rdf:resource="http://www.w3.org/2001/XMLSchema#string"/>
        <rdfs:comment xml:lang="en">hasUnit represents that a property has the name of the unit in a string.</rdfs:comment>
    </owl:DatatypeProperty>
    


    <!-- 
    ///////////////////////////////////////////////////////////////////////////////////////
    //
    // Classes
    //
    ///////////////////////////////////////////////////////////////////////////////////////
     -->

    


    <!-- http://emmo.info/domains/emmo-material.owl#EMMO_4207e895_8b83_4318_996a_72cfb32acd94 -->

    <owl:Class rdf:about="http://emmo.info/domains/emmo-material.owl#EMMO_4207e895_8b83_4318_996a_72cfb32acd94">
        <rdfs:label rdf:datatype="http://www.w3.org/2001/XMLSchema#string">Material</rdfs:label>
    </owl:Class>
    


    <!-- https://w3id.org/mdo/core/CalculatedProperty -->

    <owl:Class rdf:about="https://w3id.org/mdo/core/CalculatedProperty">
        <rdfs:subClassOf rdf:resource="https://w3id.org/mdo/core/Property"/>
        <owl:disjointWith rdf:resource="https://w3id.org/mdo/core/PhysicalProperty"/>
    </owl:Class>
    


    <!-- https://w3id.org/mdo/core/Calculation -->

    <owl:Class rdf:about="https://w3id.org/mdo/core/Calculation">
        <rdfs:subClassOf>
            <owl:Class>
                <owl:intersectionOf rdf:parseType="Collection">
                    <owl:Restriction>
                        <owl:onProperty rdf:resource="https://w3id.org/mdo/core/hasInputProperty"/>
                        <owl:someValuesFrom rdf:resource="https://w3id.org/mdo/core/Property"/>
                    </owl:Restriction>
                    <owl:Restriction>
                        <owl:onProperty rdf:resource="https://w3id.org/mdo/core/hasInputProperty"/>
                        <owl:allValuesFrom rdf:resource="https://w3id.org/mdo/core/Property"/>
                    </owl:Restriction>
                    <owl:Restriction>
                        <owl:onProperty rdf:resource="https://w3id.org/mdo/core/hasOutputCalculatedProperty"/>
                        <owl:allValuesFrom rdf:resource="https://w3id.org/mdo/core/CalculatedProperty"/>
                    </owl:Restriction>
                </owl:intersectionOf>
            </owl:Class>
        </rdfs:subClassOf>
        <rdfs:subClassOf>
            <owl:Class>
                <owl:intersectionOf rdf:parseType="Collection">
                    <owl:Restriction>
                        <owl:onProperty rdf:resource="https://w3id.org/mdo/core/hasInputStructure"/>
                        <owl:someValuesFrom rdf:resource="https://w3id.org/mdo/core/Structure"/>
                    </owl:Restriction>
                    <owl:Restriction>
                        <owl:onProperty rdf:resource="https://w3id.org/mdo/core/hasInputStructure"/>
                        <owl:allValuesFrom rdf:resource="https://w3id.org/mdo/core/Structure"/>
                    </owl:Restriction>
                    <owl:Restriction>
                        <owl:onProperty rdf:resource="https://w3id.org/mdo/core/hasOutputStructure"/>
                        <owl:allValuesFrom rdf:resource="https://w3id.org/mdo/core/Structure"/>
                    </owl:Restriction>
                </owl:intersectionOf>
            </owl:Class>
        </rdfs:subClassOf>
        <rdfs:comment xml:lang="en">A calculation is the use of a specific computational method to process structures and/or properties into output structures and/or calculated properties.</rdfs:comment>
    </owl:Class>
    


    <!-- https://w3id.org/mdo/core/PhysicalProperty -->

    <owl:Class rdf:about="https://w3id.org/mdo/core/PhysicalProperty">
        <rdfs:subClassOf rdf:resource="https://w3id.org/mdo/core/Property"/>
    </owl:Class>
    


    <!-- https://w3id.org/mdo/core/Property -->

    <owl:Class rdf:about="https://w3id.org/mdo/core/Property">
        <rdfs:comment xml:lang="en">A property in materials design is data pertaining to at least one material or materials system.</rdfs:comment>
    </owl:Class>
    


    <!-- https://w3id.org/mdo/core/Structure -->

    <owl:Class rdf:about="https://w3id.org/mdo/core/Structure">
        <rdfs:subClassOf>
            <owl:Class>
                <owl:intersectionOf rdf:parseType="Collection">
                    <owl:Restriction>
                        <owl:onProperty rdf:resource="https://w3id.org/mdo/core/relatesToMaterial"/>
                        <owl:someValuesFrom rdf:resource="http://emmo.info/domains/emmo-material.owl#EMMO_4207e895_8b83_4318_996a_72cfb32acd94"/>
                    </owl:Restriction>
                    <owl:Restriction>
                        <owl:onProperty rdf:resource="https://w3id.org/mdo/core/relatesToMaterial"/>
                        <owl:allValuesFrom rdf:resource="http://emmo.info/domains/emmo-material.owl#EMMO_4207e895_8b83_4318_996a_72cfb32acd94"/>
                    </owl:Restriction>
                </owl:intersectionOf>
            </owl:Class>
        </rdfs:subClassOf>
        <rdfs:comment xml:lang="en">A structure is the information of the sites and their occupancies in a material or materials system.</rdfs:comment>
    </owl:Class>
</rdf:RDF>



<!-- Generated by the OWL API (version 4.5.9.2019-02-01T07:24:44Z) https://github.com/owlcs/owlapi -->

