<?xml version="1.0"?>
<rdf:RDF xmlns="https://w3id.org/mdo/calculation/"
     xml:base="https://w3id.org/mdo/calculation/"
     xmlns:owl="http://www.w3.org/2002/07/owl#"
     xmlns:rdf="http://www.w3.org/1999/02/22-rdf-syntax-ns#"
     xmlns:xml="http://www.w3.org/XML/1998/namespace"
     xmlns:xsd="http://www.w3.org/2001/XMLSchema#"
     xmlns:core="https://w3id.org/mdo/core/"
     xmlns:rdfs="http://www.w3.org/2000/01/rdf-schema#"
     xmlns:vann="http://purl.org/vocab/vann/"
     xmlns:dcterms="http://purl.org/dc/terms/">
    <owl:Ontology rdf:about="https://w3id.org/mdo/calculation/">
        <owl:versionIRI rdf:resource="https://w3id.org/mdo/calculation/1.0"/>
        <owl:imports rdf:resource="https://w3id.org/mdo/core/1.0"/>
        <dcterms:contributor rdf:datatype="http://www.w3.org/2001/XMLSchema#string">Patrick Lambrix</dcterms:contributor>
        <dcterms:contributor rdf:datatype="http://www.w3.org/2001/XMLSchema#string">Rickard Armiento</dcterms:contributor>
        <dcterms:created>2019-11-07</dcterms:created>
        <dcterms:creator rdf:datatype="http://www.w3.org/2001/XMLSchema#string">Huanyu Li</dcterms:creator>
        <dcterms:license>https://github.com/huanyu-li/Materials-Design-Ontology/blob/master/LICENSE</dcterms:license>
        <dcterms:title xml:lang="en">Materials Design Ontology - Calculation Module</dcterms:title>
        <vann:preferredNamespacePrefix>calculation</vann:preferredNamespacePrefix>
        <vann:preferredNamespaceUri rdf:datatype="http://www.w3.org/2001/XMLSchema#string">https://w3id.org/mdo/calculation/1.0</vann:preferredNamespaceUri>
        <rdfs:comment xml:lang="en">This is the calculation module of Materials Design Ontology.</rdfs:comment>
        <rdfs:seeAlso>https://github.com/huanyu-li/Materials-Design-Ontology</rdfs:seeAlso>
        <owl:versionInfo rdf:datatype="http://www.w3.org/2001/XMLSchema#string">1.0</owl:versionInfo>
    </owl:Ontology>
    


    <!-- 
    ///////////////////////////////////////////////////////////////////////////////////////
    //
    // Annotation properties
    //
    ///////////////////////////////////////////////////////////////////////////////////////
     -->

    


    <!-- http://purl.org/dc/terms/contributor -->

    <owl:AnnotationProperty rdf:about="http://purl.org/dc/terms/contributor"/>
    


    <!-- http://purl.org/dc/terms/created -->

    <owl:AnnotationProperty rdf:about="http://purl.org/dc/terms/created"/>
    


    <!-- http://purl.org/dc/terms/creator -->

    <owl:AnnotationProperty rdf:about="http://purl.org/dc/terms/creator"/>
    


    <!-- http://purl.org/dc/terms/license -->

    <owl:AnnotationProperty rdf:about="http://purl.org/dc/terms/license"/>
    


    <!-- http://purl.org/dc/terms/title -->

    <owl:AnnotationProperty rdf:about="http://purl.org/dc/terms/title"/>
    


    <!-- http://purl.org/vocab/vann/preferredNamespacePrefix -->

    <owl:AnnotationProperty rdf:about="http://purl.org/vocab/vann/preferredNamespacePrefix"/>
    


    <!-- http://purl.org/vocab/vann/preferredNamespaceUri -->

    <owl:AnnotationProperty rdf:about="http://purl.org/vocab/vann/preferredNamespaceUri"/>
    


    <!-- 
    ///////////////////////////////////////////////////////////////////////////////////////
    //
    // Object Properties
    //
    ///////////////////////////////////////////////////////////////////////////////////////
     -->

    


    <!-- https://w3id.org/mdo/calculation/hasComputationalMethod -->

    <owl:ObjectProperty rdf:about="https://w3id.org/mdo/calculation/hasComputationalMethod">
        <rdfs:domain rdf:resource="https://w3id.org/mdo/core/Calculation"/>
        <rdfs:range rdf:resource="https://w3id.org/mdo/calculation/ComputationalMethod"/>
        <rdfs:comment xml:lang="en">hasComputationalMethod represents the relationship between a calculation and a computational method it uses.</rdfs:comment>
        <rdfs:label xml:lang="en">has computational method</rdfs:label>
    </owl:ObjectProperty>
    


    <!-- https://w3id.org/mdo/calculation/hasParameter -->

    <owl:ObjectProperty rdf:about="https://w3id.org/mdo/calculation/hasParameter">
        <rdfs:domain rdf:resource="https://w3id.org/mdo/calculation/ComputationalMethod"/>
        <rdfs:range rdf:resource="https://w3id.org/mdo/calculation/ComputationalMethodParameter"/>
        <rdfs:comment xml:lang="en">hasParameter represents the relationship between a calculation and the parameters it has.</rdfs:comment>
        <rdfs:label xml:lang="en">has parameter</rdfs:label>
    </owl:ObjectProperty>
    


    <!-- https://w3id.org/mdo/calculation/hasXCFunctional -->

    <owl:ObjectProperty rdf:about="https://w3id.org/mdo/calculation/hasXCFunctional">
        <rdfs:domain rdf:resource="https://w3id.org/mdo/calculation/DensityFunctionalTheoryMethod"/>
        <rdfs:range rdf:resource="https://w3id.org/mdo/calculation/ExchangeCorrelationEnergyFunctional"/>
        <rdfs:comment xml:lang="en">hasXCFunctional represents the relationship between a density functional theory method and the exchange-correlation energy functionals it takes.</rdfs:comment>
        <rdfs:label xml:lang="en">has XC functional</rdfs:label>
    </owl:ObjectProperty>
    


    <!-- 
    ///////////////////////////////////////////////////////////////////////////////////////
    //
    // Data properties
    //
    ///////////////////////////////////////////////////////////////////////////////////////
     -->

    


    <!-- https://w3id.org/mdo/calculation/ParameterName -->

    <owl:DatatypeProperty rdf:about="https://w3id.org/mdo/calculation/ParameterName">
        <rdfs:domain rdf:resource="https://w3id.org/mdo/calculation/ComputationalMethodParameter"/>
        <rdfs:range rdf:resource="http://www.w3.org/2001/XMLSchema#string"/>
        <rdfs:comment xml:lang="en">ParameterName represents that a computational method parameter has the name in a string.</rdfs:comment>
        <rdfs:label xml:lang="en">parameter name</rdfs:label>
    </owl:DatatypeProperty>
    


    <!-- https://w3id.org/mdo/calculation/ParameterValue -->

    <owl:DatatypeProperty rdf:about="https://w3id.org/mdo/calculation/ParameterValue">
        <rdfs:domain rdf:resource="https://w3id.org/mdo/calculation/ComputationalMethodParameter"/>
        <rdfs:range rdf:resource="http://www.w3.org/2001/XMLSchema#string"/>
        <rdfs:comment xml:lang="en">ParameterValue represents that a computational method parameter has the value in a string.</rdfs:comment>
        <rdfs:label xml:lang="en">parameter value</rdfs:label>
    </owl:DatatypeProperty>
    


    <!-- 
    ///////////////////////////////////////////////////////////////////////////////////////
    //
    // Classes
    //
    ///////////////////////////////////////////////////////////////////////////////////////
     -->

    


    <!-- https://w3id.org/mdo/calculation/ComputationalMethod -->

    <owl:Class rdf:about="https://w3id.org/mdo/calculation/ComputationalMethod">
        <rdfs:subClassOf>
            <owl:Class>
                <owl:intersectionOf rdf:parseType="Collection">
                    <owl:Restriction>
                        <owl:onProperty rdf:resource="https://w3id.org/mdo/calculation/hasParameter"/>
                        <owl:someValuesFrom rdf:resource="https://w3id.org/mdo/calculation/ComputationalMethodParameter"/>
                    </owl:Restriction>
                    <owl:Restriction>
                        <owl:onProperty rdf:resource="https://w3id.org/mdo/calculation/hasParameter"/>
                        <owl:allValuesFrom rdf:resource="https://w3id.org/mdo/calculation/ComputationalMethodParameter"/>
                    </owl:Restriction>
                </owl:intersectionOf>
            </owl:Class>
        </rdfs:subClassOf>
        <rdfs:comment xml:lang="en">A computational method is a way to process structures and/or properties into output structures and/or calculated properties.</rdfs:comment>
        <rdfs:label xml:lang="en">Computational Method</rdfs:label>
    </owl:Class>
    


    <!-- https://w3id.org/mdo/calculation/ComputationalMethodParameter -->

    <owl:Class rdf:about="https://w3id.org/mdo/calculation/ComputationalMethodParameter">
        <rdfs:comment xml:lang="en">A computational method parameter is a parameter used in a computational method.</rdfs:comment>
        <rdfs:label xml:lang="en">Computational Method Parameter</rdfs:label>
    </owl:Class>
    


    <!-- https://w3id.org/mdo/calculation/DensityFunctionalTheoryMethod -->

    <owl:Class rdf:about="https://w3id.org/mdo/calculation/DensityFunctionalTheoryMethod">
        <rdfs:subClassOf rdf:resource="https://w3id.org/mdo/calculation/ComputationalMethod"/>
        <rdfs:subClassOf>
            <owl:Class>
                <owl:intersectionOf rdf:parseType="Collection">
                    <owl:Restriction>
                        <owl:onProperty rdf:resource="https://w3id.org/mdo/calculation/hasXCFunctional"/>
                        <owl:someValuesFrom rdf:resource="https://w3id.org/mdo/calculation/ExchangeCorrelationEnergyFunctional"/>
                    </owl:Restriction>
                    <owl:Restriction>
                        <owl:onProperty rdf:resource="https://w3id.org/mdo/calculation/hasXCFunctional"/>
                        <owl:allValuesFrom rdf:resource="https://w3id.org/mdo/calculation/ExchangeCorrelationEnergyFunctional"/>
                    </owl:Restriction>
                </owl:intersectionOf>
            </owl:Class>
        </rdfs:subClassOf>
        <rdfs:comment xml:lang="en">A DFT method is a computational quantum mechanical modelling method used to investigate the electronic structure based on optimization of the energy over electronic densities.</rdfs:comment>
        <rdfs:label xml:lang="en">Density Functional Theory Method</rdfs:label>
    </owl:Class>
    


    <!-- https://w3id.org/mdo/calculation/ExchangeCorrelationEnergyFunctional -->

    <owl:Class rdf:about="https://w3id.org/mdo/calculation/ExchangeCorrelationEnergyFunctional">
        <rdfs:comment xml:lang="en">An ExchangeCorrelationEnergyFunctional is a functional to compute the exchange correlation energy.</rdfs:comment>
        <rdfs:label xml:lang="en">Exchange Correlation Energy Functional</rdfs:label>
    </owl:Class>
    


    <!-- https://w3id.org/mdo/calculation/GeneralizedGradientApproximation -->

    <owl:Class rdf:about="https://w3id.org/mdo/calculation/GeneralizedGradientApproximation">
        <rdfs:subClassOf rdf:resource="https://w3id.org/mdo/calculation/ExchangeCorrelationEnergyFunctional"/>
        <rdfs:comment xml:lang="en">A GeneralizedGradientApproximation is a classification of exchange correlation energy functionals that only use the local value of the electronic density and its gradient.</rdfs:comment>
        <rdfs:label xml:lang="en">Generalized Gradient Approximation</rdfs:label>
    </owl:Class>
    


    <!-- https://w3id.org/mdo/calculation/HartreeFockMethod -->

    <owl:Class rdf:about="https://w3id.org/mdo/calculation/HartreeFockMethod">
        <rdfs:subClassOf rdf:resource="https://w3id.org/mdo/calculation/ComputationalMethod"/>
        <rdfs:comment xml:lang="en">A Hartree Fock method is a computational quantum mechanical modelling method used to investigate the electronic structure based on variational search over wave functions.</rdfs:comment>
        <rdfs:label xml:lang="en">Hartree Fock Method</rdfs:label>
    </owl:Class>
    


    <!-- https://w3id.org/mdo/calculation/HybridFunctional -->

    <owl:Class rdf:about="https://w3id.org/mdo/calculation/HybridFunctional">
        <rdfs:subClassOf rdf:resource="https://w3id.org/mdo/calculation/ExchangeCorrelationEnergyFunctional"/>
        <rdfs:comment xml:lang="en">A hybrid functional is a classification of exchange correlation energy functionals that combine exact exchange from HartreeFock theory with another exchange correlation energy approximation.</rdfs:comment>
        <rdfs:label xml:lang="en">Hybrid Functional</rdfs:label>
    </owl:Class>
    


    <!-- https://w3id.org/mdo/calculation/HybridGeneralizedGradientApproximation -->

    <owl:Class rdf:about="https://w3id.org/mdo/calculation/HybridGeneralizedGradientApproximation">
        <rdfs:subClassOf rdf:resource="https://w3id.org/mdo/calculation/HybridFunctional"/>
        <rdfs:comment xml:lang="en">A hybrid generalized gradient approximation is a classification of exchange correlation energy functionals that combine exact exchange from Hartree–Fock theory with generalized gradient approximation.</rdfs:comment>
        <rdfs:label xml:lang="en">Hybrid Generalized Gradient Approximation</rdfs:label>
    </owl:Class>
    


    <!-- https://w3id.org/mdo/calculation/HybridmetaGeneralizedGradientApproximation -->

    <owl:Class rdf:about="https://w3id.org/mdo/calculation/HybridmetaGeneralizedGradientApproximation">
        <rdfs:subClassOf rdf:resource="https://w3id.org/mdo/calculation/HybridFunctional"/>
        <rdfs:comment xml:lang="en">A hybrid meta generalized gradient approximation is a classification of exchange correlation energy functionals that combine exact exchange from Hartree–Fock theory with meta generalized gradient approximation.</rdfs:comment>
        <rdfs:label xml:lang="en">Hybrid meta Generalized Gradient Approximation</rdfs:label>
    </owl:Class>
    


    <!-- https://w3id.org/mdo/calculation/LocalDensityApproximation -->

    <owl:Class rdf:about="https://w3id.org/mdo/calculation/LocalDensityApproximation">
        <rdfs:subClassOf rdf:resource="https://w3id.org/mdo/calculation/ExchangeCorrelationEnergyFunctional"/>
        <rdfs:comment xml:lang="en">An LDA is a classification of exchange correlation energy functionals that only use the local value of the electronic density.</rdfs:comment>
        <rdfs:label xml:lang="en">Local Density Approximation</rdfs:label>
    </owl:Class>
    


    <!-- https://w3id.org/mdo/calculation/metaGeneralizedGradientApproximation -->

    <owl:Class rdf:about="https://w3id.org/mdo/calculation/metaGeneralizedGradientApproximation">
        <rdfs:subClassOf rdf:resource="https://w3id.org/mdo/calculation/ExchangeCorrelationEnergyFunctional"/>
        <rdfs:comment xml:lang="en">A metaGeneralizedGradientApproximation is a classification of exchange correlation energy functionals that only use the local value of the electronic density and its gradient and the Kohn–Sham orbital kinetic energy density.</rdfs:comment>
        <rdfs:label xml:lang="en">meta Generalized Gradient Approximation</rdfs:label>
    </owl:Class>
    


    <!-- https://w3id.org/mdo/core/Calculation -->

    <owl:Class rdf:about="https://w3id.org/mdo/core/Calculation">
        <rdfs:subClassOf>
            <owl:Restriction>
                <owl:onProperty rdf:resource="https://w3id.org/mdo/calculation/hasComputationalMethod"/>
                <owl:qualifiedCardinality rdf:datatype="http://www.w3.org/2001/XMLSchema#nonNegativeInteger">1</owl:qualifiedCardinality>
                <owl:onClass rdf:resource="https://w3id.org/mdo/calculation/ComputationalMethod"/>
            </owl:Restriction>
        </rdfs:subClassOf>
    </owl:Class>
</rdf:RDF>



<!-- Generated by the OWL API (version 4.5.9.2019-02-01T07:24:44Z) https://github.com/owlcs/owlapi -->

